src/SlabsFree.fst
@@ -488,6 +488,7 @@ let deallocate_slab_aux_1
     same_base_array arr' ptr /\
     0 <= diff /\
     diff < U32.v page_size /\
+    (diff % U32.v page_size) % U32.v size_class == 0 /\
     US.v pos2 == diff /\
     US.v md_count_v <> AL.null /\
     sel md_count h0 == md_count_v /\
@@ -963,6 +964,7 @@ let deallocate_slab_aux_2
     same_base_array arr' ptr /\
     0 <= diff /\
     diff < U32.v page_size /\
+    (diff % U32.v page_size) % U32.v size_class == 0 /\
     US.v pos2 == diff /\
     US.v md_count_v <> AL.null /\
     sel md_count h0 == md_count_v /\
@@ -1173,6 +1175,7 @@ let deallocate_slab'
       (US.v idx1) (US.v idx2) (US.v idx3) (US.v idx4) (US.v idx5) h0 in
     let diff' = A.offset (A.ptr_of ptr) - A.offset (A.ptr_of slab_region) in
     0 <= diff' /\
+    (diff' % U32.v page_size) % U32.v size_class == 0 /\
     //UP.v diff < US.v metadata_max * U32.v page_size /\
     US.v diff == diff' /\
     same_base_array ptr slab_region /\
@@ -1269,6 +1272,7 @@ let deallocate_slab
   (requires fun _ ->
     let diff' = A.offset (A.ptr_of ptr) - A.offset (A.ptr_of slab_region) in
     0 <= diff' /\
+    (diff' % U32.v page_size) % U32.v size_class == 0 /\
     US.v diff_ == diff' /\
     same_base_array ptr slab_region /\
     A.length ptr == U32.v size_class)
